WIP validators with arrayptr

src/lowparse/LowParse.SteelSel.VParse.fst
@@ -4,26 +4,53 @@ include LowParse.Spec.Base
 module S = Steel.Memory
 module SE = Steel.SelEffect
 module A = Steel.SelArray
+module AP = Steel.SelArrayPtr
+
+let is_byte_repr_injective
+  #k #t p x b1 b2
+= parse_injective p b1 b2
+
+let cvalid
+  (#k: parser_kind)
+  (#t: Type)
+  (p: parser k t)
+  (c: AP.v byte)
+: Tot prop
+= valid p c.AP.contents
+
+unfold
+let intro_cvalid
+  (a: byte_array)
+  (#k: parser_kind)
+  (#t: Type)
+  (p: parser k t)
+  (c: AP.v byte)
+  (sq: squash (cvalid p c))
+: Tot (SE.t_of (AP.varrayptr a `SE.vrefine` cvalid p))
+= c
 
 let select
-  (n: Ghost.erased nat)
+  (a: byte_array)
   (#k: parser_kind)
   (#t: Type)
   (p: parser k t)
-  (x: Seq.lseq byte n { valid n p x })
-: GTot t
+  (x: SE.t_of (AP.varrayptr a `SE.vrefine` cvalid p))
+: GTot (v t)
 =
-  let Some (y, _) = parse p x in
-  y
+  let Some (y, _) = parse p x.AP.contents in
+  {
+    array = x.AP.array;
+    contents = y;
+  }
 
 let select_correct
-  (n: Ghost.erased nat)
+  (a: byte_array)
   (#k: parser_kind)
   (#t: Type)
   (p: parser k t)
-  (x: Seq.lseq byte n { valid n p x })
+  (x: SE.t_of (AP.varrayptr a `SE.vrefine` cvalid p))
 : Lemma
-  (is_byte_repr n p (select n p x) x)
+  (is_byte_repr p (select a p x).contents x.AP.contents)
 = ()
 
 let vparse0
@@ -31,8 +58,22 @@ let vparse0
   (#t: Type)
   (p: parser k t)
   (a: byte_array)
-: Tot SE.vprop
-= (A.varray a `SE.vrefine` valid (A.length a) p) `SE.vrewrite`  select (A.length a) p
+: Pure SE.vprop
+  (requires True)
+  (ensures (fun y -> SE.t_of y == v t))
+= (AP.varrayptr a `SE.vrefine` cvalid p) `SE.vrewrite`  select a p
+
+unfold
+let vparse0_sel
+  (#p:SE.vprop)
+  (#k: parser_kind) (#t: Type) (q: parser k t)
+  (r:byte_array)
+  (h:SE.rmem p{FStar.Tactics.with_tactic SE.selector_tactic (SE.can_be_split p (vparse0 q r) /\ True)})
+: GTot (v t)
+= let x : (SE.t_of (vparse0 q r)) =
+    h (vparse0 q r)
+  in
+  x
 
 let intro_vparse0
   (#k: parser_kind)
@@ -40,20 +81,21 @@ let intro_vparse0
   (p: parser k t)
   (a: byte_array)
 : SE.SteelSel unit
-    (A.varray a)
+    (AP.varrayptr a)
     (fun _ -> vparse0 p a)
     (fun h ->
-      valid (A.length a) p (h (A.varray a))
+      valid p (h (AP.varrayptr a)).AP.contents
     )
     (fun h _ h' ->
-      valid (A.length a) p (h (A.varray a)) /\
-      is_byte_repr (A.length a) p (h' (vparse0 p a)) (h (A.varray a))
+      valid p (h (AP.varrayptr a)).AP.contents /\
+      (vparse0_sel p a h').array == (h (AP.varrayptr a)).AP.array /\
+      is_byte_repr p (vparse0_sel p a h').contents (h (AP.varrayptr a)).AP.contents
     )
 =
-  SE.intro_vrefine (A.varray a) (valid (A.length a) p);
-  SE.intro_vrewrite (A.varray a `SE.vrefine` valid (A.length a) p) (select (A.length a) p);
-  assert_norm ((A.varray a `SE.vrefine` valid (A.length a) p) `SE.vrewrite` select (A.length a) p == vparse0 p a);
-  SE.change_equal_slprop ((A.varray a `SE.vrefine` valid (A.length a) p) `SE.vrewrite` select (A.length a) p) (vparse0 p a)
+  SE.intro_vrefine (AP.varrayptr a) (cvalid p);
+  SE.intro_vrewrite (AP.varrayptr a `SE.vrefine` cvalid p) (select a p);
+  assert_norm ((AP.varrayptr a `SE.vrefine` cvalid p) `SE.vrewrite` select a p == vparse0 p a); // FIXME: WHY WHY WHY?
+  SE.change_equal_slprop ((AP.varrayptr a `SE.vrefine` cvalid p) `SE.vrewrite` select a p) (vparse0 p a)
 
 let change_equal_slprop (p q: SE.vprop)
   (sq: squash (p == q))
@@ -67,23 +109,24 @@ let elim_vparse0
   (a: byte_array)
 : SE.SteelSel unit
     (vparse0 p a)
-    (fun _ -> A.varray a)
+    (fun _ -> AP.varrayptr a)
     (fun _ -> True)
     (fun h _ h' ->
-      valid (A.length a) p (h' (A.varray a)) /\
-      is_byte_repr (A.length a) p (h (vparse0 p a)) (h' (A.varray a))
+      (h' (AP.varrayptr a)).AP.array == (vparse0_sel p a h).array /\
+      valid p (h' (AP.varrayptr a)).AP.contents /\
+      is_byte_repr p (vparse0_sel p a h).contents (h' (AP.varrayptr a)).AP.contents
     )
 =
-  let sq : squash (vparse0 #k #t p a == (A.varray a `SE.vrefine` valid (A.length a) p) `SE.vrewrite` select (A.length a) p) =
-    assert_norm (vparse0 #k #t p a == (A.varray a `SE.vrefine` valid (A.length a) p) `SE.vrewrite` select (A.length a) p)
+  let sq : squash (vparse0 #k #t p a == (AP.varrayptr a `SE.vrefine` cvalid p) `SE.vrewrite` select a p) =
+    assert_norm (vparse0 #k #t p a == (AP.varrayptr a `SE.vrefine` cvalid p) `SE.vrewrite` select a p)
   in
   change_equal_slprop (vparse0 #k #t p a)
-    ((A.varray a `SE.vrefine` valid (A.length a) p) `SE.vrewrite` select (A.length a) p)
+    ((AP.varrayptr a `SE.vrefine` cvalid p) `SE.vrewrite` select a p)
     sq;
-  SE.elim_vrewrite (A.varray a `SE.vrefine` valid (A.length a) p) (select (A.length a) p);
-  let m1 = SE.get #(A.varray a `SE.vrefine` valid (A.length a) p) () in
-  assert (valid (A.length a) p (m1 (A.varray a `SE.vrefine` valid (A.length a) p)));
-  SE.elim_vrefine (A.varray a) (valid (A.length a) p)
+  SE.elim_vrewrite (AP.varrayptr a `SE.vrefine` cvalid p) (select a p);
+  let g = SE.gget (AP.varrayptr a `SE.vrefine` cvalid p) in
+  assert (valid p (Ghost.reveal g).AP.contents);
+  SE.elim_vrefine (AP.varrayptr a) (cvalid p)
 
 let vparse_slprop
   #k #t p a
@@ -99,24 +142,19 @@ let intro_vparse
   #k #t p a
 =
   intro_vparse0 p a;
-  let m = SE.get #(vparse0 p a) () in
-  let x : Ghost.erased t = m (vparse0 p a) in
-  SE.change_slprop
+  SE.change_slprop_rel
     (vparse0 p a)
     (vparse p a)
-    x
-    x
-    (fun _ -> ())
+    (fun (x: SE.t_of (vparse0 p a)) (y: SE.t_of (vparse p a)) -> (x <: v t) == y)
+    (fun _ -> ());
+  ()
 
 let elim_vparse
   #k #t p a
 =
-  let m = SE.get #(vparse p a) () in
-  let x : Ghost.erased t = m (vparse p a) in
-  SE.change_slprop
+  SE.change_slprop_rel
     (vparse p a)
     (vparse0 p a)
-    x
-    x
+    (fun (x: SE.t_of (vparse p a)) (y: SE.t_of (vparse0 p a)) -> (x <: v t) == y)
     (fun _ -> ());
   elim_vparse0 p a
