src/lowparse/LowParse.SteelSel.Validate.fst
@@ -1,30 +1,265 @@
 module LowParse.SteelSel.Validate
 include LowParse.SteelSel.VParse
+include LowParse.Low.ErrorCode
 
 module S = Steel.Memory
 module SE = Steel.SelEffect
 module A = Steel.SelArray
+module AP = Steel.SelArrayPtr
 
 module U32 = FStar.UInt32
+module U64 = FStar.UInt64
 
-noeq
-type valid_res_t : Type0 = {
-  v_contents: byte_array;
-  v_rest: byte_array;
-  v_rest_len: (v_rest_len: U32.t { U32.v v_rest_len == A.length v_rest });
-}
+(* A validator consuming the whole input buffer. Useful for all
+   parsers that do not have the strong prefix property, in particular
+   those marked ConsumesAll. *)
 
-[@SE.__steel_reduce__]
-let valid_res_vprop
+let tvalid_res_vprop
   (#t: Type0)
   (#k: parser_kind)
   (p: parser k t)
   (a: byte_array)
-  (res: option valid_res_t)
+  (res: bool)
 : Tot SE.vprop
-= match res with
-  | None -> A.varray a
-  | Some _ -> vparse p (Some?.v res).v_contents `SE.star` A.varray (Some?.v res).v_rest
+= if res
+  then vparse p a
+  else AP.varrayptr a
+
+unfold
+let tvalid_res_vprop_true
+  (#t: Type0)
+  (#k: parser_kind)
+  (p: parser k t)
+  (a: byte_array)
+  (res: bool)
+  (x: SE.t_of (tvalid_res_vprop p a res))
+: Pure (v t)
+  (requires (res == true))
+  (ensures (fun _ -> True))
+= x
+
+unfold
+let tvalid_res_vprop_false
+  (#t: Type0)
+  (#k: parser_kind)
+  (p: parser k t)
+  (a: byte_array)
+  (res: bool)
+  (x: SE.t_of (tvalid_res_vprop p a res))
+: Pure (AP.v byte)
+  (requires (res == false))
+  (ensures (fun _ -> True))
+= x
+
+let tvalidator
+  (#t: Type0)
+  (#k: parser_kind)
+  (p: parser k t)
+: Tot Type
+=
+  (a: byte_array) ->
+  (len: U32.t) ->
+  SE.SteelSel bool
+    (AP.varrayptr a)
+    (tvalid_res_vprop p a)
+    (fun h -> U32.v len == A.length (h (AP.varrayptr a)).AP.array)
+    (fun h res h' ->
+      let s = h (AP.varrayptr a) in
+      let s' = h' (tvalid_res_vprop p a res) in
+      (res == true <==> valid p s.AP.contents) /\
+      begin if res
+      then
+        let s' = tvalid_res_vprop_true p a res s' in
+        s'.array == s.AP.array /\
+        is_byte_repr p s'.contents s.AP.contents
+      else
+        let s' = tvalid_res_vprop_false p a res s' in
+        s' == s
+      end
+    )
+
+(* A validator that returns the number of bytes consumed. Contrary to
+   LowParse.Low validators, this validator can be used only if the
+   parser has the "weak prefix property" (TODO): if a parser does not
+   consume all bytes from some input buffer, then it does not depend on
+   any bytes past what it consumed.
+ *)
+
+let wvalidator
+  (#t: Type0)
+  (#k: parser_kind)
+  (p: parser k t)
+: Tot Type
+=
+  (a: byte_array) ->
+  (len: U32.t) ->
+  SE.SteelSel U64.t
+    (AP.varrayptr a)
+    (fun _ -> AP.varrayptr a)
+    (fun h -> U32.v len == A.length (h (AP.varrayptr a)).AP.array)
+    (fun h res h' ->
+      let s = h (AP.varrayptr a) in
+      h' (AP.varrayptr a) == s /\
+      begin if is_error res
+      then
+        None? (parse p s.AP.contents)
+      else
+        U64.v res <= Seq.length s.AP.contents /\
+        valid p (Seq.slice s.AP.contents 0 (U64.v res))
+      end
+    )
+
+let wvalidate_vprop
+  (#t: Type0)
+  (#k: parser_kind)
+  (p: parser k t)
+  (a: byte_array)
+  (res: option byte_array)
+: Tot SE.vprop
+= if Some? res
+  then vparse p a `SE.star` AP.varrayptr (Some?.v res)
+  else AP.varrayptr a
+
+unfold
+let wvalidate_vprop_some
+  (#t: Type0)
+  (#k: parser_kind)
+  (p: parser k t)
+  (a: byte_array)
+  (res: option byte_array)
+  (x: SE.t_of (wvalidate_vprop p a res))
+: Pure (v t & AP.v byte)
+  (requires (Some? res))
+  (ensures (fun _ -> True))
+= x
+
+unfold
+let wvalidate_vprop_none
+  (#t: Type0)
+  (#k: parser_kind)
+  (p: parser k t)
+  (a: byte_array)
+  (res: option byte_array)
+  (x: SE.t_of (wvalidate_vprop p a res))
+: Pure (AP.v byte)
+  (requires (None? res))
+  (ensures (fun _ -> True))
+= x
+
+let wvalidate_post // FIXME: WHY WHY WHY do I need to define this postcondition separately? (if not, then dummy fails to verify)
+  (#t: Type0)
+  (#k: parser_kind)
+  (p: parser k t)
+  (a: byte_array)
+  (len: U32.t)
+  (res: option byte_array)
+  (s: AP.v byte)
+  (s': SE.t_of (wvalidate_vprop p a res))
+: Tot prop
+=
+  if None? res
+  then
+    None? (parse p s.AP.contents) /\
+    wvalidate_vprop_none p a res s' == s
+  else
+    let v = wvalidate_vprop_some p a res s' in
+    let vl = fst v in
+    let vr = snd v in
+    let consumed = A.length vl.array in
+    len == A.len s.AP.array /\
+    A.merge_into vl.array vr.AP.array s.AP.array /\
+    A.length vl.array == consumed /\
+    is_byte_repr p vl.contents (Seq.slice s.AP.contents 0 consumed) /\
+    vr.AP.contents == Seq.slice s.AP.contents consumed (U32.v len)
+
+val wvalidate
+  (#t: Type0)
+  (#k: parser_kind)
+  (#p: parser k t)
+  (w: wvalidator p)
+  (a: byte_array)
+  (len: U32.t)
+: SE.SteelSel (option byte_array)
+    (AP.varrayptr a)
+    (wvalidate_vprop p a)
+    (fun h -> len == A.len (h (AP.varrayptr a)).AP.array)
+    (fun h res h' ->
+      let s = h (AP.varrayptr a) in
+      let s'  = h' (wvalidate_vprop p a res) in
+      wvalidate_post p a len res s s'
+    )
+
+let wvalidate
+  #t #k #p w a len
+=
+  let consumed = w a len in
+  if is_success consumed
+  then begin
+    let ar = AP.split a (uint64_to_uint32 consumed) in
+    intro_vparse p a;
+    let res = Some ar in
+    SE.reveal_star (vparse p a) (AP.varrayptr ar);
+    SE.change_equal_slprop
+      (vparse p a `SE.star` AP.varrayptr ar)
+      (wvalidate_vprop p a res);
+    res
+  end else begin
+    SE.noop ();
+    SE.change_equal_slprop
+      (AP.varrayptr a)
+      (wvalidate_vprop p a None);
+    None
+  end
+
+let dummy
+  (#t: Type0)
+  (#k: parser_kind)
+  (#p: parser k t)
+  (w: wvalidator p)
+  (a: byte_array)
+  (len: U32.t)
+: SE.SteelSel unit
+    (AP.varrayptr a)
+    (fun _ -> AP.varrayptr a)
+    (fun h -> len == A.len (h (AP.varrayptr a)).AP.array)
+    (fun h _ h' ->
+      h' (AP.varrayptr a) == h (AP.varrayptr a)
+    )
+=
+  let g0 : Ghost.erased (AP.v byte) = SE.gget (AP.varrayptr a) in
+  let res = wvalidate w a len in
+  if None? res
+  then begin
+    SE.noop ();
+    SE.change_equal_slprop
+      (wvalidate_vprop p a res)
+      (AP.varrayptr a)
+  end else begin
+    let ar = Some?.v res in
+    SE.change_equal_slprop
+      (wvalidate_vprop p a res)
+      (vparse p a `SE.star` AP.varrayptr ar);
+    SE.reveal_star (vparse p a) (AP.varrayptr ar);
+    let g1 : Ghost.erased (v t) = SE.gget (vparse p a) in
+    elim_vparse p a;
+    let g2 = SE.gget (AP.varrayptr a) in
+    let glen = Ghost.hide (A.length (Ghost.reveal g1).array) in
+    is_byte_repr_injective p (Ghost.reveal g1).contents (Seq.slice (Ghost.reveal g0).AP.contents 0 (Ghost.reveal glen)) (Ghost.reveal g2).AP.contents;
+    Seq.lemma_split (Ghost.reveal g0).AP.contents (Ghost.reveal glen);
+    AP.join a ar
+  end
+
+(*
+      match parse p s, res with
+      | None, None ->
+        h' (A.varray a) == s
+      | Some (v, consumed), Some res ->
+//        v == (h' (vparse p res.v_contents) <: t) /\
+//        h' (A.varray res.v_rest) == Seq.slice s consumed (A.length a) /\
+        A.merge_into res.v_contents res.v_rest a
+      | _ -> False
+    )
+  
 
 let validator
   (#t: Type0)
